Add ContLanguage

clang/lang.v
@@ -1,107 +1,369 @@
-From iris.program_logic Require Export ectx_language ectxi_language.
+From iris_os.clang Require Export cont_lang.
+From iris.algebra Require Export ofe.
+From iris.prelude Require Export strings.
 From iris.prelude Require Import gmap.
-From iris_os.clang Require Import Integers.
 Set Default Proof Using "Type".
 
+Module heap_lang.
 Open Scope Z_scope.
 
-(* Memory *)
-Definition block_id := positive.
-Definition offset := Z.
-Definition addr : Set := block_id * offset.
-Definition addrval : Set := block_id * int32.
+(** Expressions and vals. *)
+Definition loc := positive. (* Really, any countable type. *)
 
-Inductive memval :=
-| Undef: memval
-| Byte: byte → memval
-| Pointer: block_id → int32 → nat → memval
-| MNull: memval.
+Inductive base_lit : Set :=
+  | LitInt (n : Z) | LitBool (b : bool) | LitUnit | LitLoc (l : loc).
+Inductive un_op : Set :=
+  | NegOp | MinusUnOp.
+Inductive bin_op : Set :=
+  | PlusOp | MinusOp | LeOp | LtOp | EqOp.
 
-Definition mem := gmap addr memval.
+Inductive binder := BAnon | BNamed : string → binder.
+Delimit Scope binder_scope with bind.
+Bind Scope binder_scope with binder.
+Definition cons_binder (mx : binder) (X : list string) : list string :=
+  match mx with BAnon => X | BNamed x => x :: X end.
+Infix ":b:" := cons_binder (at level 60, right associativity).
+Instance binder_eq_dec_eq : EqDecision binder.
+Proof. solve_decision. Defined.
+
+Instance set_unfold_cons_binder x mx X P :
+  SetUnfold (x ∈ X) P → SetUnfold (x ∈ mx :b: X) (BNamed x = mx ∨ P).
+Proof.
+  constructor. rewrite -(set_unfold (x ∈ X) P).
+  destruct mx; rewrite /= ?elem_of_cons; naive_solver.
+Qed.
+
+(* First-order language *)
 
 Inductive val :=
-| Vundef
-| Vnull
-| Vint32: int → val
-| Vptr: addrval → val.
+| LitV (l : base_lit).
 
-Definition ident := Z.
+Bind Scope val_scope with val.
 
-Inductive type :=
-| Tnull | Tvoid | Tint8 | Tint16 | Tint32
-| Tptr: type → type
-| Tcom_ptr: ident → type
-| Tarray: type → nat → type
-| Tstruct: ident → list (ident * type) → type.
+Inductive expr :=
+  | Var (x : string)
+  | Let (x: string) (e1 e2: expr)
+  (* Base types and their operations *)
+  | Lit (l : base_lit)
+  | UnOp (op : un_op) (e : expr)
+  | BinOp (op : bin_op) (e1 e2 : expr)
+  | If (e0 e1 e2 : expr)
+  (* Concurrency *)
+  | Fork (e : expr)
+  (* Heap *)
+  | Alloc (e : expr)
+  | Load (e : expr)
+  | Store (e1 : expr) (e2 : expr)
+  | CAS (e0 : expr) (e1 : expr) (e2 : expr)
+  (* Procedure *)
+  | Ret (e: expr)
+  | Call (f: string) (vs: list val).
 
-Definition decllist := list (ident * type).
+Bind Scope expr_scope with expr.
 
-Inductive uop :=
- | oppsite
- | negation.
+Fixpoint is_closed (X : list string) (e : expr) : bool :=
+  match e with
+  | Var x => bool_decide (x ∈ X)
+  | Let x e1 e2 => is_closed ((BNamed x) :b: X) e2
+  | Lit _ => true
+  | UnOp _ e | Fork e | Alloc e | Load e =>
+     is_closed X e
+  | BinOp _ e1 e2 | Store e1 e2 =>
+     is_closed X e1 && is_closed X e2
+  | If e0 e1 e2 | CAS e0 e1 e2 =>
+     is_closed X e0 && is_closed X e1 && is_closed X e2
+  | Ret e => is_closed X e
+  | Call _ _ => true
+  end.
 
-Inductive bop :=
- | oplus | ominus | omulti | odiv | olshift | orshift
- | oand | oor | obitand | obitor | oeq | olt.
+Class Closed (X : list string) (e : expr) := closed : is_closed X e.
+Instance closed_proof_irrel env e : ProofIrrel (Closed env e).
+Proof. rewrite /Closed. apply _. Qed.
+Instance closed_decision env e : Decision (Closed env e).
+Proof. rewrite /Closed. apply _. Qed.
 
-Definition env := gmap ident (block_id * type).
+Fixpoint of_val (v : val) : expr :=
+  match v with
+  | LitV l => Lit l
+  end.
 
-(* Language *)
+Fixpoint to_val (e : expr) : option val :=
+  match e with
+  | Lit l => Some (LitV l)
+  | _ => None
+  end.
 
-(** Expression **)
-Inductive expr:=
- | enull : expr
- | evar : ident -> expr
- | econst32 : int32 -> expr
- | eunop : uop -> expr -> expr
- | ebinop : bop -> expr -> expr -> expr
- | ederef : expr -> expr
- | eaddrof : expr -> expr 
- | efield : expr -> ident -> expr
- | ecast : expr -> type -> expr
- | earrayelem : expr -> expr -> expr.  (* expr1 [ expr2 ] *)
+(** The state: heaps of vals. *)
+Definition state := gmap loc val.
 
-Inductive stmts :=
- | sskip : option val -> stmts
- | sassign : expr -> expr -> stmts (* expr1 = expr2 *)
- | sif : expr -> stmts -> stmts -> stmts (* if ( expr ) stmts1 else stmts2 *)
- | sifthen : expr -> stmts -> stmts
- | swhile : expr -> stmts -> stmts
- | sret : stmts
- | srete : expr -> stmts
- | scall : ident -> list expr -> stmts
- | scalle : expr -> ident -> list expr -> stmts
- | sseq : stmts -> stmts -> stmts (* right associative *)
- | sprint : expr -> stmts
- | sfexec : ident -> list val -> list type -> stmts
- | sfree : list (block_id * type) -> option val -> stmts
- | salloc : list val -> decllist -> stmts.
+(** Equality and other typeclass stuff *)
+Lemma to_of_val v : to_val (of_val v) = Some v.
+Proof.
+  by induction v; simplify_option_eq; repeat f_equal; try apply (proof_irrel _).
+Qed.
 
+Lemma of_to_val e v : to_val e = Some v → of_val v = e.
+Proof.
+  revert v; induction e; intros v ?; simplify_option_eq; auto with f_equal.
+Qed.
 
-Inductive exprcont:=
-| kenil : exprcont
-| keop1 : uop -> type -> exprcont -> exprcont
-| keop2r : bop -> expr -> type -> type -> exprcont -> exprcont
-| keop2l: bop -> val -> type -> type ->exprcont -> exprcont
-| kederef : type -> exprcont -> exprcont 
-| keoffset: int32 -> exprcont -> exprcont
-| kearrbase: expr -> type -> exprcont -> exprcont
-| kearrindex: val -> type -> exprcont -> exprcont
-| kecast: type -> type -> exprcont -> exprcont.
+Instance of_val_inj : Inj (=) (=) of_val.
+Proof. by intros ?? Hv; apply (inj Some); rewrite -!to_of_val Hv. Qed.
 
-Inductive stmtcont:=
-| kstop : stmtcont
-| kseq : stmts -> stmtcont -> stmtcont
-| kcall : ident -> stmts -> env -> stmtcont -> stmtcont
-| kassignr: expr -> type -> stmtcont -> stmtcont
-| kassignl : val -> type -> stmtcont -> stmtcont
-| kfuneval : ident -> list val -> list type -> list expr -> stmtcont -> stmtcont
-| kif : stmts -> stmts -> stmtcont -> stmtcont
-| kwhile : expr -> stmts -> stmtcont -> stmtcont
-| kret : stmtcont -> stmtcont.
+Instance base_lit_eq_dec : EqDecision base_lit.
+Proof. solve_decision. Defined.
+Instance un_op_eq_dec : EqDecision un_op.
+Proof. solve_decision. Defined.
+Instance bin_op_eq_dec : EqDecision bin_op.
+Proof. solve_decision. Defined.
+Instance val_eq_dec : EqDecision val.
+Proof. solve_decision. Defined.
+Instance expr_eq_dec : EqDecision expr.
+Proof. solve_decision. Defined.
 
-Inductive cureval:=
-|cure : expr -> cureval
-|curs : stmts -> cureval.
+Instance expr_inhabited : Inhabited expr := populate (Lit LitUnit).
+Instance val_inhabited : Inhabited val := populate (LitV LitUnit).
 
+Canonical Structure stateC := leibnizC state.
+Canonical Structure valC := leibnizC val.
+Canonical Structure exprC := leibnizC expr.
 
+(** Evaluation contexts *)
+Inductive ectx_item :=
+  | LetCtx (x: string) (e2 : expr)
+  | UnOpCtx (op : un_op)
+  | BinOpLCtx (op : bin_op) (e2 : expr)
+  | BinOpRCtx (op : bin_op) (v1 : val)
+  | IfCtx (e1 e2 : expr)
+  | AllocCtx
+  | LoadCtx
+  | StoreLCtx (e2 : expr)
+  | StoreRCtx (v1 : val)
+  | CasLCtx (e1 : expr) (e2 : expr)
+  | CasMCtx (v0 : val) (e2 : expr)
+  | CasRCtx (v0 : val) (v1 : val).
+
+Definition fill_item (Ki : ectx_item) (e : expr) : expr :=
+  match Ki with
+  | LetCtx x e2 => Let x e e2
+  | UnOpCtx op => UnOp op e
+  | BinOpLCtx op e2 => BinOp op e e2
+  | BinOpRCtx op v1 => BinOp op (of_val v1) e
+  | IfCtx e1 e2 => If e e1 e2
+  | AllocCtx => Alloc e
+  | LoadCtx => Load e
+  | StoreLCtx e2 => Store e e2 
+  | StoreRCtx v1 => Store (of_val v1) e
+  | CasLCtx e1 e2 => CAS e e1 e2
+  | CasMCtx v0 e2 => CAS (of_val v0) e e2
+  | CasRCtx v0 v1 => CAS (of_val v0) (of_val v1) e
+  end.
+
+(** Substitution *)
+Fixpoint subst (x : string) (es : expr) (e : expr)  : expr :=
+  match e with
+  | Var y => if decide (x = y) then es else Var y
+  | Let y e1 e2 =>
+     Let y e1 $ if decide (x ≠ y) then subst x es e2 else e2
+  | Lit l => Lit l
+  | UnOp op e => UnOp op (subst x es e)
+  | BinOp op e1 e2 => BinOp op (subst x es e1) (subst x es e2)
+  | If e0 e1 e2 => If (subst x es e0) (subst x es e1) (subst x es e2)
+  | Fork e => Fork (subst x es e)
+  | Alloc e => Alloc (subst x es e)
+  | Load e => Load (subst x es e)
+  | Store e1 e2 => Store (subst x es e1) (subst x es e2)
+  | CAS e0 e1 e2 => CAS (subst x es e0) (subst x es e1) (subst x es e2)
+  | Ret e => Ret (subst x es e)
+  | Call f vs => Call f vs (* Should we substitute f? ... useful? *)
+  end.
+
+Definition subst' (mx : binder) (es : expr) : expr → expr :=
+  match mx with BNamed x => subst x es | BAnon => id end.
+
+(** The stepping relation *)
+Definition un_op_eval (op : un_op) (v : val) : option val :=
+  match op, v with
+  | NegOp, LitV (LitBool b) => Some $ LitV $ LitBool (negb b)
+  | MinusUnOp, LitV (LitInt n) => Some $ LitV $ LitInt (- n)
+  | _, _ => None
+  end.
+
+Definition bin_op_eval (op : bin_op) (v1 v2 : val) : option val :=
+  match op, v1, v2 with
+  | PlusOp, LitV (LitInt n1), LitV (LitInt n2) => Some $ LitV $ LitInt (n1 + n2)
+  | MinusOp, LitV (LitInt n1), LitV (LitInt n2) => Some $ LitV $ LitInt (n1 - n2)
+  | LeOp, LitV (LitInt n1), LitV (LitInt n2) => Some $ LitV $ LitBool $ bool_decide (n1 ≤ n2)
+  | LtOp, LitV (LitInt n1), LitV (LitInt n2) => Some $ LitV $ LitBool $ bool_decide (n1 < n2)
+  | EqOp, v1, v2 => Some $ LitV $ LitBool $ bool_decide (v1 = v2)
+  | _, _, _ => None
+  end.
+
+Inductive head_step : expr → state → expr → state → list (expr) → Prop :=
+  | LetS x e1 e2 v1 σ e' :
+     to_val e1 = Some v1 →
+     Closed (BNamed x :b: []) e2 →
+     e' = subst' (BNamed x) (of_val v1) e2 →
+     head_step (Let x e1 e2) σ e' σ []
+  | UnOpS op e v v' σ :
+     to_val e = Some v →
+     un_op_eval op v = Some v' → 
+     head_step (UnOp op e) σ (of_val v') σ []
+  | BinOpS op e1 e2 v1 v2 v' σ :
+     to_val e1 = Some v1 → to_val e2 = Some v2 →
+     bin_op_eval op v1 v2 = Some v' → 
+     head_step (BinOp op e1 e2) σ (of_val v') σ []
+  | IfTrueS e1 e2 σ :
+     head_step (If (Lit $ LitBool true) e1 e2) σ e1 σ []
+  | IfFalseS e1 e2 σ :
+     head_step (If (Lit $ LitBool false) e1 e2) σ e2 σ []
+  | ForkS e σ:
+     head_step (Fork e) σ (Lit LitUnit) σ [e]
+  | AllocS e v σ l :
+     to_val e = Some v → σ !! l = None →
+     head_step (Alloc e) σ (Lit $ LitLoc l) (<[l:=v]>σ) []
+  | LoadS l v σ :
+     σ !! l = Some v →
+     head_step (Load (Lit $ LitLoc l)) σ (of_val v) σ []
+  | StoreS l e v σ :
+     to_val e = Some v → is_Some (σ !! l) →
+     head_step (Store (Lit $ LitLoc l) e) σ (Lit LitUnit) (<[l:=v]>σ) []
+  | CasFailS l e1 v1 e2 v2 vl σ :
+     to_val e1 = Some v1 → to_val e2 = Some v2 →
+     σ !! l = Some vl → vl ≠ v1 →
+     head_step (CAS (Lit $ LitLoc l) e1 e2) σ (Lit $ LitBool false) σ []
+  | CasSucS l e1 v1 e2 v2 σ :
+     to_val e1 = Some v1 → to_val e2 = Some v2 →
+     σ !! l = Some v1 →
+     head_step (CAS (Lit $ LitLoc l) e1 e2) σ (Lit $ LitBool true) (<[l:=v2]>σ) [].
+
+Fixpoint substs' xs vs e :=
+  match xs, vs with
+    | x::xs, v::vs => subst' (BNamed x) (of_val v) (substs' xs vs e)
+    | _, _ => e
+  end.
+
+Definition fundecls : Type := string → (list string * expr).
+
+Definition cont : Type := list ectx_item.
+
+Inductive cont_step : fundecls → expr → ectx_item → cont → expr → cont → Prop :=
+| CallK:
+    ∀ decls f xs vs K ks e e',
+      decls f = (xs, e) →
+      length xs = length vs →
+      e' = substs' xs vs e →
+      cont_step decls (Call f vs) K ks e' (K::ks)
+| RetK:
+    ∀ decls e v K k ks,
+      to_val e = Some v →
+      cont_step decls (Ret e) K (k::ks) (fill_item k e) ks.
+
+(** Basic properties about the language *)
+Instance fill_item_inj Ki : Inj (=) (=) (fill_item Ki).
+Proof. destruct Ki; intros ???; simplify_eq/=; auto with f_equal. Qed.
+
+Lemma fill_item_val Ki e :
+  is_Some (to_val (fill_item Ki e)) → is_Some (to_val e).
+Proof. intros [v ?]. destruct Ki; simplify_option_eq; eauto. Qed.
+
+Lemma val_stuck e1 σ1 e2 σ2 efs : head_step e1 σ1 e2 σ2 efs → to_val e1 = None.
+Proof. destruct 1; naive_solver. Qed.
+
+Lemma head_ctx_step_val Ki e σ1 e2 σ2 efs :
+  head_step (fill_item Ki e) σ1 e2 σ2 efs → is_Some (to_val e).
+Proof. destruct Ki; inversion_clear 1; simplify_option_eq; by eauto. Qed.
+
+Lemma fill_item_no_val_inj Ki1 Ki2 e1 e2 :
+  to_val e1 = None → to_val e2 = None →
+  fill_item Ki1 e1 = fill_item Ki2 e2 → Ki1 = Ki2.
+Proof.
+  destruct Ki1, Ki2; intros; try discriminate; simplify_eq/=;
+    repeat match goal with
+    | H : to_val (of_val _) = None |- _ => by rewrite to_of_val in H
+    end; auto.
+Qed.
+
+Lemma alloc_fresh e v σ :
+  let l := fresh (dom _ σ) in
+  to_val e = Some v → head_step (Alloc e) σ (Lit (LitLoc l)) (<[l:=v]>σ) [].
+Proof. by intros; apply AllocS, (not_elem_of_dom (D:=gset _)), is_fresh. Qed.
+
+(* Misc *)
+
+(** Closed expressions *)
+Lemma is_closed_weaken X Y e : is_closed X e → X ⊆ Y → is_closed Y e.
+Proof. revert X Y; induction e; naive_solver (eauto; set_solver). Qed.
+
+Lemma is_closed_weaken_nil X e : is_closed [] e → is_closed X e.
+Proof. intros. by apply is_closed_weaken with [], list_subseteq_nil. Qed.
+
+Lemma is_closed_of_val X v : is_closed X (of_val v).
+Proof. apply is_closed_weaken_nil. induction v; simpl; auto. Qed.
+
+Lemma is_closed_subst X e x es :
+  is_closed [] es → is_closed (x :: X) e → is_closed X (subst x es e).
+Proof.
+  intros ?. revert X.
+  induction e=> X /= ?; destruct_and?; split_and?; simplify_option_eq;
+    try match goal with
+    | H : ¬(_ ∧ _) |- _ => apply not_and_l in H as [?%dec_stable|?%dec_stable]
+    end; eauto using is_closed_weaken with set_solver.
+Qed.
+Lemma is_closed_do_subst' X e x es :
+  is_closed [] es → is_closed (x :b: X) e → is_closed X (subst' x es e).
+Proof. destruct x; eauto using is_closed_subst. Qed.
+
+(* Substitution *)
+Lemma subst_is_closed X e x es : is_closed X e → x ∉ X → subst x es e = e.
+Proof.
+  revert X. induction e=> X /=; rewrite ?bool_decide_spec ?andb_True=> ??;
+    repeat case_decide; simplify_eq/=; f_equal; intuition eauto with set_solver.
+Qed.
+
+Lemma subst_is_closed_nil e x es : is_closed [] e → subst x es e = e.
+Proof. intros. apply subst_is_closed with []; set_solver. Qed.
+
+Lemma subst_subst e x es es' :
+  Closed [] es' → subst x es (subst x es' e) = subst x es' e.
+Proof.
+  intros. induction e; simpl; try (f_equal; by auto);
+    simplify_option_eq; auto using subst_is_closed_nil with f_equal.
+Qed.
+Lemma subst_subst' e x es es' :
+  Closed [] es' → subst' x es (subst' x es' e) = subst' x es' e.
+Proof. destruct x; simpl; auto using subst_subst. Qed.
+
+Lemma subst_subst_ne e x y es es' :
+  Closed [] es → Closed [] es' → x ≠ y →
+  subst x es (subst y es' e) = subst y es' (subst x es e).
+Proof.
+  intros. induction e; simpl; try (f_equal; by auto);
+    simplify_option_eq; auto using eq_sym, subst_is_closed_nil with f_equal.
+Qed.
+Lemma subst_subst_ne' e x y es es' :
+  Closed [] es → Closed [] es' → x ≠ y →
+  subst' x es (subst' y es' e) = subst' y es' (subst' x es e).
+Proof. destruct x, y; simpl; auto using subst_subst_ne with congruence. Qed.
+
+End heap_lang.
+
+(** Language *)
+Program Instance heap_cont_lang :
+  ContLanguage
+    (heap_lang.expr) heap_lang.val heap_lang.ectx_item
+    heap_lang.state heap_lang.fundecls heap_lang.cont := {|
+  of_val := heap_lang.of_val; to_val := heap_lang.to_val;
+  fill := heap_lang.fill_item; head_step := heap_lang.head_step;
+  cont_step := heap_lang.cont_step
+|}.
+Solve Obligations with eauto using heap_lang.to_of_val, heap_lang.of_to_val,
+  heap_lang.val_stuck, heap_lang.fill_item_val, heap_lang.fill_item_no_val_inj,
+  heap_lang.head_ctx_step_val.
+
+(* Prefer heap_lang names over ectx_language names. *)
+Export heap_lang.
+
+(** Define some derived forms *)
+Notation Seq e1 e2 := (Let BAnon e1 e2).
+Notation Skip := (Seq (Lit LitUnit) (Lit LitUnit)).
